vevictb

steel/Veritas.Steel.Verifier.fsti
@@ -9,10 +9,26 @@ module U64 = FStar.UInt64
 open Veritas.Steel.VCache
 open Veritas.Steel.Types
 open Steel.Reference
+
+
+module MSH = Veritas.MultiSetHashDomain
+let model_hash = erased MSH.mset_ms_hashfn_dom
+
+[@@erasable]
+noeq
+type thread_state_model = {
+  model_failed : bool;
+  model_store  : VCache.contents;
+  model_clock  : erased U64.t;
+  model_hadd   : model_hash;
+  model_hevict : model_hash;
+}
+
+val prf_set_hash : Type0
+val prf_set_hash_inv (_:prf_set_hash) (_:model_hash) : slprop u#1
+
 let thread_id = U32.t
 let counter_t = ref U64.t
-val prf_set_hash : Type0
-val prf_set_hash_inv (_:prf_set_hash) : slprop u#1
 
 noeq
 type thread_state_t = {
@@ -24,21 +40,16 @@ type thread_state_t = {
   failed       : ref bool
 }
 
-[@@erasable]
-noeq
-type thread_state_model = {
-  model_failed : bool;
-  model_store : VCache.contents;
-  model_clock : erased U64.t;
-//add sets to model hash state
-}
-
 [@@__reduce__]
 let thread_state_inv (t:thread_state_t) (m:thread_state_model)
   : slprop
   = VCache.is_vstore t.st m.model_store `star`
-    pts_to t.clock full_perm m.model_clock `star`
-    pts_to t.failed full_perm m.model_failed
+    //NS: it actually seems to matter that I associate it explicitly this way
+    //which is odd. See failure in vget if you remove the parentheses
+    (pts_to t.clock full_perm m.model_clock `star`
+     (pts_to t.failed full_perm m.model_failed `star`
+      (prf_set_hash_inv t.hadd m.model_hadd `star`
+       prf_set_hash_inv t.hevict m.model_hevict)))
 
 let change_slprop (#[@@framing_implicit] p:slprop)
                   (#[@@framing_implicit] q:slprop)
@@ -67,6 +78,13 @@ let vget_model tsm (s:slot tsm) (v:value) : thread_state_model =
   | Some r' ->
     if v = r'.record_value then tsm else model_fail tsm
 
+let emp_unit (p:slprop)
+  : Lemma ((p `star` emp == p) /\
+           (emp `star` p == p))
+          [SMTPatOr [[SMTPat (p `star` emp)];
+                     [SMTPat (emp `star` p)]]]
+  = admit()
+
 let vget (#tsm:_) (s:slot tsm) (v:value) (vs: thread_state_t)
   : SteelT unit
     (requires thread_state_inv vs tsm)
@@ -75,12 +93,12 @@ let vget (#tsm:_) (s:slot tsm) (v:value) (vs: thread_state_t)
     match ro with
     | None ->
       fail vs "Slot not found";
-      change_slprop ()
+      rewrite_context ()
     | Some r' ->
       if v = r'.record_value
-      then (change_slprop #(thread_state_inv vs tsm) #(thread_state_inv vs (vget_model tsm s v)) (); ())
+      then rewrite_context ()
       else (fail vs "Failed: inconsistent key or value in Get";
-            change_slprop())
+            rewrite_context ())
 
 let model_get_record (tsm:thread_state_model) (s:slot tsm)
   : GTot (option record)
@@ -89,6 +107,10 @@ let model_get_record (tsm:thread_state_model) (s:slot tsm)
 let model_put_record (tsm:thread_state_model) (s:slot tsm) (r:record)
   : thread_state_model
   = {tsm with model_store=Seq.upd tsm.model_store (U32.v s) (Some r)}
+
+let model_evict_record (tsm:thread_state_model) (s:slot tsm)
+  : thread_state_model
+  = {tsm with model_store=Seq.upd tsm.model_store (U32.v s) None }
 
 let vput_model (tsm:thread_state_model) (s:slot tsm) (v:value)
   : thread_state_model
@@ -104,29 +126,44 @@ let vput (#tsm:_) (s:slot tsm) (v:value) (vs: thread_state_t)
   = let ro = VCache.vcache_get_record vs.st s in
     match ro with
     | None ->
-      let _ = fail vs "Slot not found" in
-      change_slprop()
+      let _ = fail #tsm vs "Slot not found" in
+      //Same as in vcache_set, but this time we have emps on both sides
+      rewrite_context ()
 
     | Some r ->
       let x = vcache_update_record vs.st s ({ r with record_value = v }) in
-      change_slprop #(is_vstore _ _ `star` pts_to vs.clock _ _ `star` pts_to vs.failed _ _)// (Mkthread_state_t?.st vs)
-                      //           (hide (Seq.Base.upd (reveal (Mkthread_state_model?.model_store tsm))
-                      //                               (UInt32.v s)
-                      //                               (Some (update_record_value r v)))) `star`
-                      // Steel.Reference.pts_to (Mkthread_state_t?.clock vs)
-                      //                        full_perm
-                      //                        (Mkthread_state_model?.model_clock tsm))
-                    #(thread_state_inv vs (vput_model tsm s v))
-                    ()
+      rewrite_context #(is_vstore _ _ `star` (pts_to vs.clock _ _ `star` (pts_to vs.failed _ _ `star` _)))
+                      #(thread_state_inv _ _)
+                      ()
 
 val epoch_of_timestamp (t:timestamp) : U32.t
 
-val model_update_hash (tsm:thread_state_model) (r:record) (t:timestamp) (thread_id:thread_id)
-  : tsm':thread_state_model{tsm.model_store == tsm'.model_store}
-val update_hash (#tsm:_) (r:record) (t:timestamp) (thread_id:thread_id) (vs:thread_state_t)
+
+val mk_mhdom (r:record) (t:timestamp) (thread_id:thread_id) : MSH.ms_hashfn_dom
+
+val model_update_hash (h:model_hash) (r:record) (t:timestamp) (thread_id:thread_id)
+  : model_hash
+
+val prf_update_hash (#m:model_hash) (p:prf_set_hash) (r:record) (t:timestamp) (thread_id:thread_id)
+  : SteelT unit
+    (prf_set_hash_inv p m)
+    (fun _ -> prf_set_hash_inv p (model_update_hash m r t thread_id))
+
+let model_update_hadd (tsm:_) (r:record) (t:timestamp) (thread_id:thread_id) =
+  ({tsm with model_hadd = model_update_hash tsm.model_hadd r t thread_id})
+
+val update_hadd (#tsm:_) (r:record) (t:timestamp) (thread_id:thread_id) (vs:thread_state_t)
   : SteelT unit
     (thread_state_inv vs tsm)
-    (fun _ -> thread_state_inv vs (model_update_hash tsm r t thread_id))
+    (fun _ -> thread_state_inv vs ({tsm with model_hadd = model_update_hash tsm.model_hadd r t thread_id})) //(model_update_hadd tsm r t thread_id))
+
+let model_update_hevict (tsm:_) (r:record) (t:timestamp) (thread_id:thread_id) =
+  ({tsm with model_hevict = model_update_hash tsm.model_hevict r t thread_id})
+
+val update_hevict (#tsm:_) (r:record) (t:timestamp) (thread_id:thread_id) (vs:thread_state_t)
+  : SteelT unit
+    (thread_state_inv vs tsm)
+    (fun _ -> thread_state_inv vs (model_update_hevict tsm r t thread_id))
 
 open FStar.Integers
 
@@ -145,6 +182,7 @@ let update_clock (#tsm:_) (ts:timestamp) (vs:thread_state_t)
 let mk_record k v am = { record_key = k; record_value = v; record_add_method = am;
                          record_l_child_in_store = Vfalse;
                          record_r_child_in_store = Vfalse }
+
 let vaddb_model (tsm:thread_state_model) (s:slot tsm) (r:record) (t:timestamp) (thread_id:thread_id)
   : thread_state_model
   = let e = epoch_of_timestamp t in
@@ -156,7 +194,7 @@ let vaddb_model (tsm:thread_state_model) (s:slot tsm) (r:record) (t:timestamp) (
     else (
       //TODO: need to check that the key does not exist
       (* updated h_add *)
-      let tsm = model_update_hash tsm r t thread_id in
+      let tsm = model_update_hadd tsm r t thread_id in
       (* updated clock *)
       let tsm = model_update_clock tsm t in
       (* add record to store *)
@@ -180,49 +218,104 @@ let vaddb (#tsm:_)
     if not (is_value_of k v)
     then (
       fail vs "vaddm: value is incompatible with key";
-      change_slprop #(thread_state_inv vs _)
-                    #(thread_state_inv vs _)
-                    ()
+      rewrite_context #(thread_state_inv vs _)
+                      #(thread_state_inv vs _)
+                      ()
     )
     else (
       let ro = VCache.vcache_get_record vs.st s in
       if Some? ro
       then (
         fail vs "vaddm: slot s already exists";
-        change_slprop #(thread_state_inv _ _)
-                      #(thread_state_inv _ _)
-                      ()
+        rewrite_context #(thread_state_inv _ _)
+                        #(thread_state_inv _ _)
+                        ()
       )
       else (
-        update_hash r t thread_id vs;
-        update_clock t vs;
+        prf_update_hash vs.hadd r t thread_id;// vs;
+        update_clock #(model_update_hadd tsm r t thread_id) t vs;
         //this next line is tricky for a couple of reasons
         // 1. the implicit arg to vcache_update_record is unified with the type of `s` which is indexed
         //    by the original tsm, not the current one
         // 2. the refinement type mk_record require `is_value_of k v` does not seem to be provable
         //    here. despite the check above.
         VCache.vcache_update_record #((model_update_clock _ _).model_store) vs.st s (mk_record k v BAdd);
-        change_slprop #(is_vstore _ _ `star` pts_to vs.clock _ _ `star` pts_to vs.failed _ _)
-                      #(thread_state_inv vs (vaddb_model tsm s r t thread_id))
-                      ()
+        rewrite_context #(is_vstore _ _ `star` (pts_to vs.clock _ _ `star` (pts_to vs.failed _ _ `star` _)))
+                        #(thread_state_inv vs (vaddb_model tsm s r t thread_id))
+                        ()
       )
     )
 
-// let vevictb (s:slot_id) (t:timestamp) (vs:thread_state_t)
-//   : StackExn unit
-//     (requires fun h -> thread_state_inv vs h)
-//     (ensures fun h0 _ h1 -> thread_state_inv vs h1)
-//   = let e = epoch_of_timestamp in
-//     let clk = B.index vs.clock 0ul in
-//     if not (clk `timestamp_lt` t) then raise "vevictb: timestamp does not exceed the clock";
-//     (* check that the vstore contains s *)
-//     let r = vstore_get_record vs.st s in
-//     (* update the evict hash *)
-//     multiset_hash_upd r t vs.id vs.hevict;
-//     (* advance clock to t *)
-//     update_clock t vs.clock;
-//     (* evict record *)
-//     vstore_evict_record vs.st s r.record_key
+let timestamp_lt (t0 t1:timestamp) = t0 `U64.lt` t1
+
+let vevictb_model (tsm:thread_state_model) (s:slot tsm) (t:timestamp) (thread_id:thread_id)
+  : GTot thread_state_model
+  = let e = epoch_of_timestamp t in
+    let clk = tsm.model_clock in
+    if not (clk `timestamp_lt` t)
+    then model_fail tsm
+    else begin
+      (* check that the vstore contains s *)
+      match model_get_record tsm s with
+      | None -> model_fail tsm
+      | Some r ->
+        (* update the evict hash *)
+        let tsm = model_update_hevict tsm r t thread_id in
+        (* advance clock to t *)
+        let tsm = model_update_clock tsm t in
+        (* evict record *)
+        model_evict_record tsm s
+    end
+
+let read_id (#a:Type) (#p:perm) (#v:erased a) (r:ref a)
+  : Steel a
+    (requires pts_to r p v)
+    (ensures fun _ -> pts_to r p v)
+    (requires fun _ -> True)
+    (ensures fun _ res _ -> hide res == v)
+  = let x = read r in
+    rewrite_context #(pts_to r p (hide x))
+                    #(pts_to r p v)
+                    ();
+    x
+
+
+let vevictb (#tsm:_)
+            (s:slot tsm)
+            (t:timestamp)
+            (vs:thread_state_t)
+  : SteelT unit
+    (requires thread_state_inv vs tsm)
+    (ensures fun _ -> thread_state_inv vs (vevictb_model tsm s t vs.id))
+  = let clk = read_id vs.clock in
+    if not (clk `timestamp_lt` t)
+    then (
+      fail vs "Timestamp is old";
+      rewrite_context #(thread_state_inv _ _)
+                      #(thread_state_inv _ _)
+                       ()
+    )
+    else (
+      (* check that the vstore contains s *)
+      let r = VCache.vcache_get_record vs.st s in
+      match r with
+      | None ->
+        fail vs "Slot is empty";
+        rewrite_context #(thread_state_inv _ _)
+                        #(thread_state_inv _ _)
+                        ()
+
+      | Some r ->
+        (* update the evict hash *)
+        prf_update_hash vs.hevict r t vs.id;
+
+        update_clock #(model_update_hevict tsm r t vs.id) t vs;
+
+        VCache.vcache_evict_record #((model_update_clock _ _).model_store) vs.st s;
+
+        rewrite_context #(is_vstore _ _ `star` (pts_to vs.clock _ _ `star` (pts_to vs.failed _ _ `star` _)))
+                        #(thread_state_inv vs (vevictb_model tsm s t vs.id))
+                        ())
 
 // let vevictbm (s s':slot_id) (t:timestamp) (vs:thread_state_t)
 //   : StackExn unit
